theories/Index/Index.v
@@ -8,6 +8,7 @@ Require Import DschingisKhan.Math.BasicPosetTheory.
 Require Import DschingisKhan.Math.BooleanAlgebra.
 Require Import DschingisKhan.Math.ClassicalDomainTheory.
 Require Import DschingisKhan.Math.PropositionalLogicExtra.
+Require Import DschingisKhan.Math.GIT.
 Require Import DschingisKhan.Logic.ConstructiveDomainTheory.
 Require Import DschingisKhan.Logic.InteractionTreeTheory.
 Require Import DschingisKhan.Logic.LambdaCalculus.
