theories/Math/GIT.v
@@ -1,0 +1,33 @@
+Require Import Coq.Arith.Compare_dec.
+Require Import Coq.Arith.PeanoNat.
+Require Import Coq.Bool.Bool.
+Require Import Coq.Classes.RelationClasses.
+Require Import Coq.Lists.List.
+Require Import Coq.micromega.Lia.
+Require Import Coq.Program.Basics.
+Require Import Coq.Relations.Relation_Definitions.
+Require Import Coq.Relations.Relation_Operators.
+Require Import DschingisKhan.Prelude.PreludeInit.
+Require Import DschingisKhan.Prelude.PreludeMath.
+Require Import DschingisKhan.Prelude.PreludeUtil.
+Require Import DschingisKhan.Prelude.PreludeClassic.
+Require Import DschingisKhan.Data.Vector.
+Require Import DschingisKhan.Data.InteractionTree.
+Require Import DschingisKhan.Logic.PeanoArithmetic.
+Require Import DschingisKhan.Logic.InteractionTreeTheory.
+
+Module GIT.
+
+  Import ListNotations InteractionTrees.
+
+  Local Existing Instances freeSetoidFromSetoid1.
+
+  Record isComputableFunction {arity : nat} (funGraph : ensemble (vector nat arity * nat)) : Type :=
+    { computer : vector nat arity -> itree void1 nat
+    ; computer_repr (args : vector nat arity) (rv : nat)
+      (CONVERGES : exists fuel : nat, burnTau_nat fuel (computer args) == Ret rv)
+      : forall result : nat, rv = result <-> member (args, result) funGraph
+    }
+  .
+
+End GIT.
